Setlec/Model/Annotate.lean
@@ -336,7 +336,7 @@ theorem annotateCore_sound (m : EnvModel V env) :
     have hoke₂ : FvarsOk V m.val env φ d ρ e₂ := fun l hl => hoke l (hsl l hl)
     have hAe₂ : AnnotOk V m.val env φ d ρ e₂ :=
       annotateCore_sound m fuel e he hw hb hLbe ρ hoke
-    rcases hres with ⟨us, A, B, cv, hteq, hfind, hi2, rfl⟩ | hel
+    rcases hres with ⟨us, A, B, cv, caps, hteq, hfind, hi2, rfl⟩ | hel
     case inr =>
       obtain ⟨us, pcv, nP, nM, nm, ni, rules, -, -, -,
         hwsb, hrb, hall, hann⟩ := annotateProjElim_inv hel
@@ -385,7 +385,7 @@ theorem annotateCore_sound (m : EnvModel V env) :
       rw [← hψ']
       simp only [hal, if_true]
     have hvf₀ : vf₀ = m.val psigmaName ψ' := (Option.some.inj hci).symm
-    have hfacts := ((m.ind_ok.1 cv hfind).2 ψ')
+    have hfacts := ((m.ind_ok.1 cv caps hfind).2 ψ')
     have hAmem : vA ∈ˢ univ (ψ' uN) := hfacts.dom₀ (hvf₀ ▸ hpi₀) hvA₀
     have hf₁ : vf₁ = app (m.val psigmaName ψ') vA := by
       rw [interpExpr, hval, hAi] at hf₁i
