Setlec/Verify/InferLeaves.lean
@@ -228,7 +228,7 @@ theorem whnf_fvarLeaves {env : Env} (henv : EnvWF env) :
           next hal => exact (Except.ok.inj h) ▸ fun l hl => hl
         | axiomInfo cv => exact (Except.ok.inj h) ▸ fun l hl => hl
         | thmInfo cv value => exact (Except.ok.inj h) ▸ fun l hl => hl
-        | indInfo cv => exact (Except.ok.inj h) ▸ fun l hl => hl
+        | indInfo cv _ => exact (Except.ok.inj h) ▸ fun l hl => hl
         | ctorInfo cv nP nF => exact (Except.ok.inj h) ▸ fun l hl => hl
         | recInfo cv nP nM nm ni rules => exact (Except.ok.inj h) ▸ fun l hl => hl
     | .app f a, h =>
@@ -325,7 +325,7 @@ theorem whnf_looseBVars {env : Env} (henv : EnvWF env) :
           next hal => exact (Except.ok.inj h) ▸ hb
         | axiomInfo cv => exact (Except.ok.inj h) ▸ hb
         | thmInfo cv value => exact (Except.ok.inj h) ▸ hb
-        | indInfo cv => exact (Except.ok.inj h) ▸ hb
+        | indInfo cv _ => exact (Except.ok.inj h) ▸ hb
         | ctorInfo cv nP nF => exact (Except.ok.inj h) ▸ hb
         | recInfo cv nP nM nm ni rules => exact (Except.ok.inj h) ▸ hb
     | .app f a, h =>
@@ -429,7 +429,7 @@ theorem inferTypeCore_WScoped {env : Env} (henv : EnvWF env) :
       simp only [WScoped] at hwPi
       exact WScoped.instantiate1_gen hw.2 0 hwPi.2
     | .proj sn i e, h =>
-      obtain ⟨te, us, A, B, cv2, hte, hwt, hfind2, hcase⟩ := inferTypeCore_proj_inv h
+      obtain ⟨te, us, A, B, cv2, caps2, hte, hwt, hfind2, hcase⟩ := inferTypeCore_proj_inv h
       simp only [WScoped] at hw
       have hwte := inferTypeCore_WScoped henv fuel hte hw
       have hwPi := whnf_WScoped henv fuel hwt hwte
@@ -510,7 +510,7 @@ theorem inferTypeCore_fvarLeaves {env : Env} (henv : EnvWF env) :
         simp [fvarLeaves, hb]
       · exact Or.inr hb
     | .proj sn i e, h =>
-      obtain ⟨te, us, A, B, cv2, hte, hwt, hfind2, hcase⟩ := inferTypeCore_proj_inv h
+      obtain ⟨te, us, A, B, cv2, caps2, hte, hwt, hfind2, hcase⟩ := inferTypeCore_proj_inv h
       simp only [WScoped] at hw
       intro l hl
       simp only [fvarLeaves]
@@ -593,7 +593,7 @@ theorem inferTypeCore_looseBVars {env : Env} (henv : EnvWF env) :
       simp only [looseBVarsBounded, Bool.and_eq_true] at hbPi
       exact looseBVarsBounded_instantiate1_gen hb.2 hbPi.2
     | .proj sn i e, h =>
-      obtain ⟨te, us, A, B, cv2, hte, hwt, hfind2, hcase⟩ := inferTypeCore_proj_inv h
+      obtain ⟨te, us, A, B, cv2, caps2, hte, hwt, hfind2, hcase⟩ := inferTypeCore_proj_inv h
       simp only [WScoped] at hw
       simp only [looseBVarsBounded] at hb
       have hLbe : Expr.LeavesBounded e := fun l hl => hLb l (by
